---
title: Quadratic Expressions & Equations
topic: "4048"
---
# Quadratics
An expression written in the form of $ax^2 + bx +c$ is a **quadratic expression**, whereas an equation written in the form of $ax^2+bx+c =0$ is a **quadratic equation**.
$a$ is the coefficient of $x^2$, $b$ is the coefficient of $x$, and $c$ is the constant term.
When solving a quadratic equation, we are finding the value(s) of $x$ that satisfy the equation. These solutions are known as the **root(s)** of the equation.
## Zero product property
The **zero product property** states that if $ab = 0$, then $a = 0$ or $b = 0$.
Many methods of factorisation utilise this property to factorise quadratic equations:
- by common factors
- by algebraic identities
- by trial & error (inspection)

---
# Completing the square
There are some quadratic equations which cannot be completely factorised by using methods which utilise the zero product property.
Hence, another method is to **complete the square**.
- form a perfect square from the quadratic expression on the left of the equation by introducing a constant
- solve the equation using the differences of squares approach, or the square root approach

>[!example]
> We can solve $x^2 - 6x +3=0$ by completing the square.
>$$
>\begin{align*} x^2 - 6x + 3 &= 0 \\ x^2 - 6x + \left(3^2 - 3^2\right) &= 0 \\ \left(x+3\right)^2 - 9 + 3 &= 0 \\ \left(x+3\right)^2 - 6 &= 0 \\ \left(x+3\right)^2 &= 0 \\ x+3&= \sqrt{6} \text{ or } -\sqrt6 \end{align*}
>$$
>$\therefore x = -3+\sqrt6 \text{ or } -3-\sqrt6$

For the general quadratic expression $x^2+bx$, the constant added and subtracted is $\left(\frac{b}{2}\right)^2$.

---
# Quadratic formula
The **quadratic formula** is a compressed version of completing the square, and can be used to solve virtually any quadratic equation. 
The solutions to the quadratic expression $ax^2+bx+c=0$, where $a\neq0$, are
$$
x=\frac{-b-\sqrt{b^2-4ac}}{2a}\text{ or }\frac{-b+\sqrt{b^2-4ac}}{2a}
$$

---
# Quadratic graphs
For quadratic equations in the form $y = ax^2 + bx + c = 0$ with roots $\alpha$ and $\beta$,
- $\alpha + \beta = -\frac{b}{a}$
- $\alpha\beta = \frac{c}{a}$

For quadratic equations in the form $y = a(x-\alpha)(x-\beta)$,
- the curve opens upwards if $a>0$, downwards if $a<0$
- the $x$-coordinates are $\alpha$ and $\beta$
- the $x$-coordinate of the turning point is $\frac{\alpha+\beta}{2}$

For quadratic equations in the form $y = a\left(x-h\right)^2+k$,
- the curve opens upwards if $a>0$, downwards if $a<0$
- the turning point can be found at $\left(h, k\right)$